Accessors. More validators

src/lowparse/LowParse.Low.Int.fst
@@ -1,4 +1,5 @@
 module LowParse.Low.Int
+open LowParse.Low.Combinators
 
 module Aux = LowParse.Low.Int.Aux
 module Unique = LowParse.Spec.Int.Unique
@@ -12,6 +13,7 @@ module B = FStar.Buffer
 
 #set-options "--z3rlimit 16"
 
+inline_for_extraction
 let parse32_u8 =
   (fun (input: pointer buffer8) (len: pointer U32.t) ->
     let h = HST.get () in
@@ -19,6 +21,7 @@ let parse32_u8 =
     Aux.parse32_u8 input len
   )
 
+inline_for_extraction
 let parse32_u16 =
   (fun (input: pointer buffer8) (len: pointer U32.t) ->
     let h = HST.get () in
@@ -26,9 +29,34 @@ let parse32_u16 =
     Aux.parse32_u16 input len
   )
 
+inline_for_extraction
 let parse32_u32 =
   (fun (input: pointer buffer8) (len: pointer U32.t) ->
     let h = HST.get () in
     let _ = Unique.parse_u32_unique (B.as_seq h (B.get h input 0)) in
     Aux.parse32_u32 input len
   )
+
+inline_for_extraction
+let validate32_u8 : validator32 parse_u8 =
+  validate32_total_constant_size parse_u8 1ul ()
+
+inline_for_extraction
+let validate32_u16 : validator32 parse_u16 =
+  validate32_total_constant_size parse_u16 2ul ()
+
+inline_for_extraction
+let validate32_u32 : validator32 parse_u32 =
+  validate32_total_constant_size parse_u32 4ul ()
+
+inline_for_extraction
+let validate_nochk32_u8 : validator_nochk32 parse_u8 =
+  validate_nochk32_constant_size parse_u8 1ul ()
+
+inline_for_extraction
+let validate_nochk32_u16 : validator_nochk32 parse_u16 =
+  validate_nochk32_constant_size parse_u16 2ul ()
+
+inline_for_extraction
+let validate_nochk32_u32 : validator_nochk32 parse_u32 =
+  validate_nochk32_constant_size parse_u32 4ul ()
