src/lowparse/LowParse.Low.Int.fsti
@@ -10,3 +10,21 @@ val parse32_u16: parser32 parse_u16
 
 inline_for_extraction
 val parse32_u32: parser32 parse_u32
+
+inline_for_extraction
+val validate32_u8: validator32 parse_u8
+
+inline_for_extraction
+val validate32_u16: validator32 parse_u16
+
+inline_for_extraction
+val validate32_u32: validator32 parse_u32
+
+inline_for_extraction
+val validate_nochk32_u8: validator_nochk32 parse_u8
+
+inline_for_extraction
+val validate_nochk32_u16: validator_nochk32 parse_u16
+
+inline_for_extraction
+val validate_nochk32_u32: validator_nochk32 parse_u32
